Figured out

theories/fp_red.v
@@ -22,36 +22,41 @@ Ltac spec_refl := ltac2:(spec_refl ()).
 Module ERed.
   Inductive R {n} : PTm n -> PTm n ->  Prop :=
   (****************** Eta ***********************)
-  | AppEta A a :
-    R (PAbs A (PApp (ren_PTm shift a) (VarPTm var_zero))) a
-  | PairEta a :
-    R (PPair (PProj PL a) (PProj PR a)) a
-
+  | AppEta A a0 a1 :
+    R a0 a1 ->
+    R (PAbs A (PApp (ren_PTm shift a0) (VarPTm var_zero))) a1
+  | PairEta a0 a1 :
+    R a0 a1 ->
+    R (PPair (PProj PL a0) (PProj PR a0)) a1
   (*************** Congruence ********************)
   | AbsCong A a0 a1 :
     R a0 a1 ->
     R (PAbs A a0) (PAbs A a1)
-  | AppCong0 a0 a1 b :
+  | AppCong a0 a1 b0 b1 :
     R a0 a1 ->
-    R (PApp a0 b) (PApp a1 b)
-  | AppCong1 a b0 b1 :
     R b0 b1 ->
-    R (PApp a b0) (PApp a b1)
-  | PairCong0 a0 a1 b :
+    R (PApp a0 b0) (PApp a1 b1)
+  | PairCong a0 a1 b0 b1 :
     R a0 a1 ->
-    R (PPair a0 b) (PPair a1 b)
-  | PairCong1 a b0 b1 :
     R b0 b1 ->
-    R (PPair a b0) (PPair a b1)
+    R (PPair a0 b0) (PPair a1 b1)
   | ProjCong p a0 a1 :
     R a0 a1 ->
-    R (PProj p a0) (PProj p a1).
+    R (PProj p a0) (PProj p a1)
+  | VarTm i :
+    R (VarPTm i) (VarPTm i).
+
+  Lemma refl n (a : PTm n) : R a a.
+  Proof.
+    elim : n / a; hauto lq:on ctrs:R.
+  Qed.
 
   Derive Dependent Inversion inv with (forall n (a b : PTm n), R a b) Sort Prop.
 
-  Lemma AppEta' n A a (u : PTm n) :
-    u = (PAbs A (PApp (ren_PTm shift a) (VarPTm var_zero))) ->
-    R u a.
+  Lemma AppEta' n A a0 a1 (u : PTm n) :
+    u = (PAbs A (PApp (ren_PTm shift a0) (VarPTm var_zero))) ->
+    R a0 a1 ->
+    R u a1.
   Proof. move => ->. apply AppEta. Qed.
 
   Lemma renaming n m (a b : PTm n) (ξ : fin n -> fin m) :
@@ -60,22 +65,152 @@ Module ERed.
     move => h. move : m ξ.
     elim : n a b /h.
 
-    move => n A a m ξ /=.
-    apply AppEta' with (A := A). by asimpl.
+    move => n A a0 a1 ha iha m ξ /=.
+    eapply AppEta' with (A := A); eauto. by asimpl.
     all : qauto ctrs:R.
+  Qed.
+
+  Lemma morphing_ren n m p (ρ0 ρ1 : fin n -> PTm m) (ξ : fin m -> fin p) :
+    (forall i, R (ρ0 i) (ρ1 i)) ->
+    (forall i, R ((funcomp (ren_PTm ξ) ρ0) i) ((funcomp (ren_PTm ξ) ρ1) i)).
+  Proof. eauto using renaming. Qed.
+
+  Lemma morphing_ext n m (ρ0 ρ1 : fin n -> PTm m) a b  :
+    R a b ->
+    (forall i, R (ρ0 i) (ρ1 i)) ->
+    (forall i, R ((scons a ρ0) i) ((scons b ρ1) i)).
+  Proof. hauto q:on inv:option. Qed.
+
+  Lemma morphing_up n m (ρ0 ρ1 : fin n -> PTm m) :
+    (forall i, R (ρ0 i) (ρ1 i)) ->
+    (forall i, R (up_PTm_PTm ρ0 i) (up_PTm_PTm ρ1 i)).
+  Proof. hauto l:on ctrs:R use:morphing_ext, morphing_ren unfold:up_PTm_PTm. Qed.
+
+  Lemma morphing n m (a b : PTm n) (ρ0 ρ1 : fin n -> PTm m) :
+    (forall i, R (ρ0 i) (ρ1 i)) ->
+    R a b -> R (subst_PTm ρ0 a) (subst_PTm ρ1 b).
+  Proof.
+    move => + h. move : m ρ0 ρ1. elim : n a b / h => n.
+    move => A a0 a1 ha iha m ρ0 ρ1 hρ /=.
+    eapply AppEta' with (A := A); eauto. by asimpl.
+    all : hauto lq:on ctrs:R use:morphing_up.
   Qed.
 
   Lemma substing n m (a : PTm n) b (ρ : fin n -> PTm m) :
     R a b ->
     R (subst_PTm ρ a) (subst_PTm ρ b).
   Proof.
-    move => h. move : m ρ. elim : n a b / h => n.
-    move => A a m ρ /=.
-    apply AppEta' with (A := A); eauto. by asimpl.
-    all : hauto ctrs:R inv:option use:renaming.
+    hauto l:on use:morphing, refl.
   Qed.
 
 End ERed.
+
+Inductive SNe {n} : PTm n -> Prop :=
+| N_Var i :
+  SNe (VarPTm i)
+| N_App a b :
+  SNe a ->
+  SN b ->
+  SNe (PApp a b)
+| N_Proj p a :
+  SNe a ->
+  SNe (PProj p a)
+with SN  {n} : PTm n -> Prop :=
+| N_Pair a b :
+  SN a ->
+  SN b ->
+  SN (PPair a b)
+| N_Abs A a :
+  SN a ->
+  SN (PAbs A a)
+| N_SNe a :
+  SNe a ->
+  SN a
+| N_Exp a b :
+  TRedSN a b ->
+  SN b ->
+  SN a
+with TRedSN {n} : PTm n -> PTm n -> Prop :=
+| N_β A a b :
+  SN b ->
+  TRedSN (PApp (PAbs A a) b) (subst_PTm (scons b VarPTm) a)
+| N_AppL a0 a1 b :
+  TRedSN a0 a1 ->
+  TRedSN (PApp a0 b) (PApp a1 b)
+| N_ProjPairL a b  :
+  SN b ->
+  TRedSN (PProj PL (PPair a b)) a
+| N_ProjPairR a b  :
+  SN a ->
+  TRedSN (PProj PR (PPair a b)) b
+| N_ProjCong p a b :
+  TRedSN a b ->
+  TRedSN (PProj p a) (PProj p b).
+
+Scheme sne_ind := Induction for SNe Sort Prop
+  with sn_ind := Induction for SN Sort Prop
+  with sred_ind := Induction for TRedSN Sort Prop.
+
+Combined Scheme sn_mutual from sne_ind, sn_ind, sred_ind.
+
+Check sn_mutual.
+
+Lemma ered_sn_preservation n :
+  (forall (a : PTm n) (s : SNe a), forall b, ERed.R a b -> SNe b) /\
+  (forall (a : PTm n) (s : SN a), forall b, ERed.R a b -> SN b) /\
+  (forall (a b : PTm n) (_ : TRedSN a b), forall c, ERed.R a c -> exists d, TRedSN c d /\ ERed.R b d).
+Proof.
+  move : n. apply sn_mutual => n.
+  - sauto lq:on.
+  - sauto lq:on.
+  - sauto lq:on.
+  - move => a b ha iha hb ihb b0.
+    inversion 1; subst.
+    + have /iha : (ERed.R (PProj PL a0) (PProj PL b0)) by sauto lq:on.
+      admit.
+    + sauto lq:on.
+  - move => A a ha iha b.
+    inversion 1; subst.
+    + have : ERed.R (PApp (ren_PTm shift a0) (VarPTm var_zero))  (PApp (ren_PTm shift b) (VarPTm var_zero)).
+      apply ERed.AppCong; eauto using ERed.refl.
+      sfirstorder use:ERed.renaming.
+      move /iha.
+      admit.
+    + sauto lq:on.
+  - sauto lq:on.
+  - sauto lq:on.
+  - move => A a b ha iha c h0.
+    inversion h0; subst.
+    inversion H1; subst.
+    + exists (PApp a1 b1). split. admit.
+      asimpl.
+      sauto lq:on.
+    + have  {}/iha := H3 => iha.
+      exists (subst_PTm (scons b1 VarPTm) a2).
+      split.
+      sauto lq:on.
+      hauto lq:on use:ERed.morphing, ERed.refl inv:option.
+  - sauto lq:on.
+  - move => a b hb ihb c.
+    elim /ERed.inv => //= _.
+    move => p a0 a1 ha [*]. subst.
+    elim  /ERed.inv :  ha => //= _.
+    + move => a0 a2 ha [*]. subst.
+      exists (PProj PL a1).
+      split. admit.
+      sauto lq:on.
+    + sauto lq:on rew:off.
+  - move => a b ha iha c.
+    elim /ERed.inv => //=_.
+    move => p a0 a1 + [*]. subst.
+    elim /ERed.inv => //=_.
+    + move => a0 a2 h [*]. subst.
+      exists (PProj PR a1).
+      split. admit.
+      sauto lq:on.
+    + sauto lq:on.
+  - sauto lq:on.
+Admitted.
 
 Module RRed.
   Inductive R {n} : PTm n -> PTm n ->  Prop :=
